RAC of arithmetic properties: cleanups, begining of fsl semantics

Playground.v
@@ -9,55 +9,64 @@ Open Scope string_scope.
 Open Scope Z_scope.
 
 
-Declare Scope mini_c_scope.
-
-Declare Custom Entry mini_c.
-
-Notation "<{ e }>" := e (at level 0, e custom mini_c at level 99) : mini_c_scope.
-Notation "( x )" := x (in custom mini_c, x at level 99) : mini_c_scope.
-Notation "x" := x (in custom mini_c at level 0, x constr at level 0) : mini_c_scope.
-Notation "'skip'" := Skip  (in custom mini_c at level 0) : mini_c_scope.
-Notation "'if' '(' cond ')' '{' _then '}' 'else' '{' _else '}'" := (If cond _then _else) 
-    (in custom mini_c at level 89, cond at level 99, _then at level 99, _else at level 99) : mini_c_scope.
-Notation "x + y"   := (BinOpInt x C_Add y) (in custom mini_c at level 50, left associativity) : mini_c_scope.
-Notation "s1 ';' s2" := (Seq s1 s2) (in custom mini_c at level 90, right associativity) : mini_c_scope.
-Notation "x := y" := (Assign x y) (in custom mini_c at level 0, x constr at level 0, y at level 85, no associativity) : mini_c_scope.
-
-
 Open Scope mini_c_scope. 
 Open Scope fsl_scope.
 
-
-Lemma ir5 : Int.inRange 5. Proof. split ; reflexivity. Qed.
-Lemma ir10 : Int.inRange 10. Proof. split ; reflexivity. Qed.
-Lemma ir15 : Int.inRange 15. Proof. split ; reflexivity. Qed.
+Fact ir3 : Int.inRange 3. now split. Qed.
+Fact ir5 : Int.inRange 5. now split. Qed.
+Fact ir10 : Int.inRange 10 . now split. Qed.
+Fact ir14 : Int.inRange 14. now split. Qed.
+Fact ir15 : Int.inRange 15. now split. Qed.
+Definition zero := Int.of_z 0 zeroinRange.
+Definition three := Int.of_z 3 ir3.
 Definition five := Int.of_z 5 ir5.
 Definition ten := Int.of_z 10 ir10.
 Definition fifteen := Int.of_z 15 ir15.
 
 
-Example stmt_5Plus10 :
+Example imptest :
     forall o m,     
     let v := fst o in 
     let l := snd o in 
     c_stmt_sem
+    o m 
+    
     <{
-         "x" := 5 ;
-         "y" := 10;
-         "z" := "x" + "y"
-    }>
-    o m (v{"x" \ five}{"y"\ten}{"z"\fifteen}, l) m
+        "x" := 5 ;
+        "y" := 10;
+        "z" := "x" + "y";
+        "g" := 0;
+
+        if ("z" <= 14)
+            "g" := "z"
+        else 
+            "g" := "z" / 5
+
+   }>
+    
+    (v{"x" \ five}{"y"\ten}{"z"\fifteen}{"g"\zero}{"g"\three}, l) m
    .
 Proof.
     intros.
      apply S_Seq with (v{"x" \ five},l) m.
-     apply S_Assign. apply E_Int.
+     apply S_Assign. apply C_E_Int.
      apply S_Seq with (v{"x" \ five}{"y" \ ten}, l) m.
-     - apply S_Assign. apply E_Int.
-     - apply S_Assign. apply E_BinOpInt with (z:=5) (z':=10) (z_ir:=ir5) (z'_ir:=ir10) ; apply E_Var.
-        * reflexivity.
-        * reflexivity.
+     - apply S_Assign. apply C_E_Int.
+     - apply S_Seq with (v{"x" \ five}{"y" \ ten}{"z" \ fifteen}, l) m.
+        + apply S_Assign. apply C_E_BinOpInt with (z:=5) (z':=10) (z_ir:=ir5) (z'_ir:=ir10) ; 
+          now apply C_E_Var. 
+        + apply S_Seq  with (v{"x" \ five}{"y" \ ten}{"z" \ fifteen}{"g"\ zero}, l) m. 
+          ++ apply S_Assign. apply C_E_Int.
+          ++ apply S_IfFalse with zero.
+            * apply C_E_BinOpFalse with 15 14 ir15 ir14 ; try now constructor.
+            simpl. intro H. destruct H. reflexivity.
+            * reflexivity.
+            * apply S_Assign. apply C_E_BinOpInt with  (z:=15) (z':=5) (z_ir:=ir15) (z'_ir:=ir5); now constructor.
 Qed.
 
 Close Scope mini_c_scope.
-Close Scope fsl_scope.
+
+
+
+Example test_dom : ~ dom (fun x => if x>?2 then Some (x*2) else None) 2.
+Proof. intro contra. inversion contra. destruct H. discriminate. Qed.
