Semantics.v
@@ -5,69 +5,94 @@ Require Import ZArith.ZArith.
 From Coq Require Import Strings.String.
 Open Scope fsl_scope.
 Open Scope Z_scope.
+Open Scope mini_c_scope.
 
 
-Inductive c_exp_sem : c_exp -> Ω -> Values -> Prop :=
-| E_Int (z:Z) env in_range: env ⊨ z =>  (Int.of_z z in_range)
-| E_Var (x:V) z (env:Ω) : 
+Inductive c_exp_sem (env : Ω) : c_exp -> Values -> Prop :=
+| C_E_Int (z:Z) in_range: env ⊨ z => (Int.of_z z in_range)
+| C_E_Var (x:V) z  : 
     (fst env)(x:string) = Some (Int z) -> 
     env ⊨ x => z
-| E_BinOpInt env e e' (z z':Z) op z_ir z'_ir 
+| C_E_BinOpInt e e' (z z':Z) op z_ir z'_ir 
     (H:Int.inRange (⋄ op z z')) :
     env ⊨ e =>  (Int.of_z z z_ir) ->
     env ⊨ e' =>  (Int.of_z z' z'_ir) ->
     env ⊨ BinOpInt e op e' => Int.of_z ((⋄ op) z z') H
-| E_BinOpTrue env e e' (z z' : Z) z_ir z'_ir op :
+| C_E_BinOpTrue e e' (z z' : Z) z_ir z'_ir op :
     env ⊨ e => (Int.of_z z z_ir) ->
     env ⊨ e' => (Int.of_z z z'_ir) ->
-    ((◁ op) z z' = True) ->
+    ((◁ op) z z' -> True) ->
     env ⊨ BinOpBool e op e' => Int.of_z 1 oneinRange
-| E_BinOpFalse env e e' (z z' : Z) op z_ir z'_ir :
+| C_E_BinOpFalse e e' (z z' : Z) op z_ir z'_ir :
     env ⊨ e => (Int.of_z z z_ir) -> 
     env ⊨ e' => (Int.of_z z' z'_ir) -> 
-    ((◁ op) z z' = False) ->
+    ((◁ op) z z' -> False) ->
     env ⊨ BinOpBool e op e' => Int.of_z 0 zeroinRange
 
-where  "Ω '⊨' e => v" := (c_exp_sem e Ω v).
+where  "Ω '⊨' e => v" := (c_exp_sem Ω e v).
 
 
-Inductive c_decl_sem : c_decl -> Ω -> M -> Ω -> M -> Prop := 
-    | Decl (env:Ω) (v := fst env) (l := snd env) mem t x (u:Values) : 
+Inductive c_decl_sem (env:Ω) (mem:M) : c_decl -> Ω -> M -> Prop := 
+    | Decl t x (u:Values) : 
         (* v x = ⊥ -> (env,mem ⊨ C_Decl t x => (v{x\u},l),mem) *)
-        c_decl_sem (C_Decl t x) env mem (v{x\u}, l) mem 
+        c_decl_sem  env mem (C_Decl t x) ((fst env){x\u}, snd env) mem 
   (* where 
   "Ω ',' M '⊨' d '=>' Ω' ',' M'" := (c_decl_sem d Ω M Ω' M')  *)
 .
 
 
-Inductive c_stmt_sem : S -> Ω -> M -> Ω -> M -> Prop := 
-    | S_skip env mem : c_stmt_sem Skip env mem env mem
-    | S_Assign (env:Ω) (v:= fst env) (l:= snd env) mem x z e : 
+Inductive c_stmt_sem (env:Ω) (mem:M) : S -> Ω -> M -> Prop := 
+    | S_skip  : c_stmt_sem env mem <{ skip }> env mem
+    | S_Assign x z e : 
         (* in v x Int + Uint  *)
         env ⊨ e => z ->
-        c_stmt_sem (Assign x e) env mem (v{x\z},l) mem
-    | S_IfTrue (env env':Ω) mem mem' z e s s' :
+        c_stmt_sem  env mem <{x := e}> ((fst env){x\z},snd env) mem
+    | S_IfTrue env' mem' z e s s' :
         env ⊨ e => z ->
         z <>  Int.of_z 0 zeroinRange ->
-        c_stmt_sem s env mem env' mem' ->
-        c_stmt_sem (If e s s') env mem env' mem' 
-    | S_IfFalse (env env':Ω) mem mem' z e s s' :
+        c_stmt_sem env mem s  env' mem' ->
+        c_stmt_sem  env mem <{ if (e) s else s' }> env' mem' 
+    | S_IfFalse env' mem' z e s s' :
         env ⊨ e => z ->
         z = Int.of_z 0 zeroinRange ->
-        c_stmt_sem s' env mem env' mem' ->
-        c_stmt_sem (If e s s') env mem env' mem' 
-    | S_While e s env mem env' mem' :
-        c_stmt_sem (If e (Seq s (While e s)) Skip) env mem env' mem' ->
-        c_stmt_sem (While e s) env mem env' mem' 
-    | S_Seq env mem env' mem' env'' mem'' s s' :
-        c_stmt_sem s env mem env' mem' -> 
-        c_stmt_sem s' env' mem' env'' mem'' ->
-        c_stmt_sem (Seq s s') env mem env'' mem''
-    | S_Assert env mem e z :
+        c_stmt_sem  env mem s' env' mem' ->
+        c_stmt_sem  env mem <{ if (e) s else s' }> env' mem' 
+    | S_While e s   env' mem' :
+        c_stmt_sem  env mem (If e (Seq s (While e s)) Skip) env' mem' ->
+        c_stmt_sem  env mem <{ while (e) s }> env' mem' 
+    | S_Seq  env' mem' env'' mem'' s s' :
+        c_stmt_sem  env mem s env' mem' -> 
+        c_stmt_sem  env' mem' s' env'' mem'' ->
+        c_stmt_sem env mem <{ s ; s' }>  env'' mem''
+    | S_Assert  e z :
         env ⊨ e => z -> z <>  Int.of_z 0 zeroinRange ->
-        c_stmt_sem (PAssert e) env mem env mem
+        c_stmt_sem env mem <{ assert (e) }> env mem
 
  (* where "Ω ',' M '⊨' s '=>' Ω' ',' M'" := (c_stmt_sem s Ω M Ω' M') *)
     .
 
-(* TODO: mini-fsl *)
+(* TODO: finish mini-fsl semantic *)
+
+Inductive fsl_term_sem (env:Ω) : LT -> Values -> Prop :=
+| FSL_E_Int z : fsl_term_sem env z UMpz
+| FSL_E_LVar x z : (snd env) x = Some z -> fsl_term_sem env x UMpz
+| FSL_E_Var x v : (fst env) v = Some x ->  fsl_term_sem env v x
+(* | FSL_E_BinOpInt t t' z zint z' z'int op :  
+    values_int z = Some (Int zint) ->
+    values_int z' = Some (Int z'int) ->
+    fsl_term_sem env t z ->
+    fsl_term_sem env t' z' ->
+    ~ (op = FSL_Div /\ zint = (Int (Int.mkMI 0 zeroinRange))) ->
+    fsl_term_sem env (T_BinOp t op t') ((fsl_binop_int_model op) zint z'int) *)
+.
+
+
+(* Inductive fsl_pred_sem : B -> Ω -> M -> Ω -> M -> Prop :=
+| none
+. *)
+
+(* 
+Inductive fsl_assert_sem : S -> Ω -> M -> Ω -> M -> Prop := 
+| P_Assert env mem p :  env ⊨ p => Int.of_z 1 oneinRange -> 
+    fsl_assert_sem (LAssert p) env mem env mem
+. *)
