Theorems.v
@@ -11,6 +11,100 @@ Open Scope Z_scope.
 Open Scope list_scope.
 
 
+Fact eq_env_partial_order :  forall e e' v z, e ⊑ e' ->  z <> UInt /\ z <> UMpz -> (fst e) v = Some z -> (fst e') v = Some z.
+Proof.
+    intros. destruct H with v ; try assumption ; try rewrite H2 in H1 ; try injection H1 as Eq ; subst ; try assumption.
+    - destruct H0 as [uint _]. destruct uint. reflexivity.
+    - destruct H0 as [_ umpz]. destruct umpz. reflexivity.
+    - discriminate.
+Qed.
+
+
+Lemma weakening_of_expression_semantics : 
+forall env e x,
+    env ⊨ e => x <-> (forall env', env ⊑ env' ->  env' ⊨ e => x)
+.
+Proof.
+    split.
+    - generalize dependent x. induction e.
+        * intros v H env' Inc. inversion H. subst. apply C_E_Int.
+        * intros v H env' Inc. inversion H. subst. apply C_E_Var.
+            apply eq_env_partial_order with (v:=var) (z:=z) in Inc.
+            ** assumption.
+            ** split ; intro contra ; inversion contra.
+            ** assumption.
+        * intros v H env' Inc. inversion H ;  subst. 
+            apply C_E_BinOpInt with z_ir z'_ir.
+             + apply IHe1 ; assumption.
+             + apply IHe2 ; assumption.
+        * intros. inversion H ; subst.
+            + apply C_E_BinOpTrue with z z' z_ir z'_ir.
+                ++ apply IHe1 ; assumption.
+                ++ apply IHe2 ; assumption.
+                ++ assumption.
+            + apply C_E_BinOpFalse with z z' z_ir z'_ir.
+                ++ apply IHe1 ; assumption.
+                ++ apply IHe2 ; assumption.
+                ++ assumption.
+    - intro. apply H. constructor.
+Qed.
+
+
+
+Lemma weakening_of_statement_semantics_1 :
+    forall Ω₀ M₀ s Ω₁ M₁,
+    c_stmt_sem  Ω₀ M₀ s Ω₁ M₁ <->
+    forall Ω₀' M₀', [(Ω₀ , M₀)] ⊑ [(Ω₀', M₀')] ->
+     exists Ω₁' M₁', 
+     [(Ω₁ , M₁)] ⊑ [(Ω₁', M₁')] /\  c_stmt_sem Ω₀' M₀' s Ω₁' M₁'.
+Proof.
+    split. 
+    - induction s ; intro H ; inversion H ; subst ; intros.
+        * exists Ω₀'. exists M₀'. split. apply H0. constructor.
+        * exists ((fst Ω₀'){var\z}, (snd Ω₀')). exists M₀'. destruct H0 as [H0 _]. split.
+         ** split. 
+            *** intro x. destruct Ω₀,Ω₀'. apply <- env_partial_order_next. apply (H0 x).
+            *** apply fixme.
+         ** constructor. apply (weakening_of_expression_semantics Ω₀) ; assumption.
+        * admit.
+        * admit.
+        * admit.
+        * admit.
+        * admit.
+    - intros. destruct H with Ω₀ M₀ as [Ω₀' [M₀' [[Inc fixme] H1]]]; subst; clear H. 
+        * constructor ; constructor.
+        * inversion H1 ; subst.
+            ** admit.
+             ** replace  Ω₁ with ((fst Ω₀) {x \ z}, snd Ω₀). replace M₁ with M₀' . apply S_Assign.
+               *** assumption.
+               *** admit.
+               *** admit.
+            **
+Admitted.
+
+(* 2 *)
+
+Lemma weakening_of_statement_semantics_2 :
+    forall Ω₀ Ω₀' M₀ M₀' s Ω₁ M₁,
+    c_stmt_sem  Ω₀ M₀ s Ω₁ M₁ /\ [(Ω₀ , M₀)] ⊑ [(Ω₀', M₀')]  ->
+    forall Ω₁' M₁',
+    c_stmt_sem Ω₀' M₀' s Ω₁' M₁' -> 
+    (forall (v:V), ~(dom (fst Ω₀) v) -> fst Ω₀' v = fst Ω₁' v) /\ 
+    (forall x, ~ exists (v:V), (fst Ω₀ v) = Some x -> M₀' x = M₁' x).
+Admitted.
+
+
+Lemma weakening_of_statement_semantics_3 :
+    forall Ω₀ Ω₀' M₀ M₀' s Ω₁ M₁,
+    c_stmt_sem  Ω₀ M₀ s Ω₁ M₁  ->
+    [(Ω₀' , M₀')] ⊑ [(Ω₀, M₀)] ->
+    forall v, True (* todo (dom -) (dom (fst Ω₀) - dom (fst Ω₀')) v *) -> VarNotInStmt s v -> 
+    (forall x, True (* (dom M₀ - dom M₀') x *) -> (fst Ω₀) v = x) ->
+    exists Ω₁' M₁', c_stmt_sem  Ω₀' M₀' s Ω₁' M₁'.
+
+Admitted.
+
+
 
 Theorem absence_of_dangling_pointers :
     forall n (z:=VMpz n) (mem_state:M) (var_env:Ωᵥ), 
@@ -20,43 +114,3 @@ Theorem absence_of_dangling_pointers :
 .
 Admitted.
 
-
-
-Lemma weakening_of_expression_semantics : 
-forall env e x,
-    env ⊨ e => x <-> (forall env', env ⊑ env' ->  env' ⊨ e => x)
-.
-Proof.
-    assert (
-        eq_env_partial_order : forall e e' v z, e ⊑ e' ->  z <> UInt /\ z <> UMpz -> (fst e) v = Some z -> (fst e') v = Some z
-    ). 
-    {
-        intros. destruct H with v ; try assumption ; try rewrite H2 in H1 ; try injection H1 as Eq ; subst ; try assumption.
-        - destruct H0 as [uint _]. destruct uint. reflexivity.
-        - destruct H0 as [_ umpz]. destruct umpz. reflexivity.
-        - discriminate.
-    }
-
-    split.
-    - generalize dependent x. induction e.
-        * intros v H env' Inc. inversion H. subst. apply E_Int.
-        * intros v H env' Inc. inversion H. subst. apply E_Var.
-            apply eq_env_partial_order with (v:=var) (z:=z) in Inc.
-            ** assumption.
-            ** split ; intro contra ; inversion contra.
-            ** assumption.
-        * intros v H env' Inc. inversion H ;  subst. 
-            apply E_BinOpInt with z_ir z'_ir.
-             + apply IHe1 ; assumption.
-             + apply IHe2 ; assumption.
-        * intros. inversion H ; subst.
-            + apply E_BinOpTrue with z z' z_ir z'_ir.
-                ++ apply IHe1 ; assumption.
-                ++ apply IHe2 ; assumption.
-                ++ assumption.
-            + apply E_BinOpFalse with z z' z_ir z'_ir.
-                ++ apply IHe1 ; assumption.
-                ++ apply IHe2 ; assumption.
-                ++ assumption.
-    - intro. apply H. constructor.
-Qed.
